Further cleanup of the Tree-based process scheduler refinement
The value to insert is now automatically retrieved from the formulation
of the query, allowing to prove the correction of the insertion
automatically. The "prove trivial constraints" tactic could probably be
cleaned up further, though.

ADTExamples/QueryStructure/Bags/CachingBags.v
@@ -417,45 +417,46 @@ Section CacheableFunctions.
         apply ListMax_correct.
     Qed.
 
-    Definition cached_max_gt_property {TItem} (projection: TItem -> nat) seq value cached_max :=
-      List.In value seq -> S cached_max > projection value.
+    Definition cached_gt_property {TItem} (projection: TItem -> nat) seq value cached :=
+      List.In value seq -> S cached > projection value.
 
-    Lemma cached_max_gt :
+    Definition cached_neq_property {TItem} (projection: TItem -> nat) seq value cached :=
+      List.In value seq -> S cached <> projection value.
+
+    Lemma max_cached_gt :
       forall default,
-        CacheImplementationEnsures cached_max_gt_property max default. 
+        CacheImplementationEnsures cached_gt_property max default. 
     Proof.
-      unfold CacheImplementationEnsures, cached_max_gt_property; 
+      unfold CacheImplementationEnsures, cached_gt_property; 
       intros;
       destruct (ListMax_correct seq default) as (sup & _);
       apply Gt.le_gt_S, sup;
       simpl; auto.
     Qed.
 
-    Lemma cached_max_gt_projected' {TItem} projection :
+    Lemma max_cached_gt_projected {TItem} projection : 
       forall default,
-        ProjectedCacheImplementationEnsures_strong (TItem := TItem) cached_max_gt_property 
-                                                   max projection default.
+        ProjectedCacheImplementationEnsures (TItem := TItem) cached_gt_property max projection default.
     Proof.
-      unfold ProjectedCacheImplementationEnsures.
-      unfold cached_max_gt_property.
- 
-      intros;
-      apply (generalize_to_projection projection default cached_max_gt_property (cached_max_gt default)).
-    Qed.
-
-    Lemma cached_max_gt_projected {TItem} projection : 
-      forall default,
-        ProjectedCacheImplementationEnsures (TItem := TItem) cached_max_gt_property max projection default.
-    Proof.
-      intros.
-      pose proof (generalize_to_projection projection default cached_max_gt_property (cached_max_gt default)) as H.
-
       unfold 
         ProjectedCacheImplementationEnsures_strong, 
         ProjectedCacheImplementationEnsures,
-        cached_max_gt_property in *;
+        cached_gt_property in *;
+      intros;
+      apply (generalize_to_projection projection default cached_gt_property (max_cached_gt default));
+      apply in_map_unproject; 
+      assumption.
+    Qed.
+
+    Lemma max_cached_neq_projected {TItem} projection : 
+      forall default,
+        ProjectedCacheImplementationEnsures (TItem := TItem) cached_neq_property max projection default.
+    Proof.
+      unfold 
+        ProjectedCacheImplementationEnsures,
+        cached_neq_property in *;
       intros; 
-      apply H, in_map_unproject; 
+      apply gt_neq_impl, max_cached_gt_projected; 
       assumption.
     Qed.
   End MaxCacheable.
